A'_{0} = |A_{-1}|^2[Re(T^{0}_{-1,-1,0})Re(T^{0}_{-1,-1,0}) + Im(T^{0}_{-1,-1,0})Im(T^{0}_{-1,-1,0})] \\ 
\omega_{0} = 2[(2*0 + 1)(2*0+1)d^{0}_{0,0}*d^{0}_{0,0}*d^{1}_{-1,-1}*d^{1}_{-1,-1}] \\
 \\ 
A'_{1} = |A_{1}|^2[Re(T^{0}_{-1,-1,0})Re(T^{0}_{-1,-1,0}) + Im(T^{0}_{-1,-1,0})Im(T^{0}_{-1,-1,0})] \\ 
\omega_{1} = 2[(2*0 + 1)(2*0+1)d^{0}_{0,0}*d^{0}_{0,0}*d^{1}_{-1,1}*d^{1}_{-1,1}] \\
 \\ 
A'_{2} = |A_{-1}|^2[Re(T^{0}_{1,1,0})Re(T^{0}_{1,1,0}) + Im(T^{0}_{1,1,0})Im(T^{0}_{1,1,0})] \\ 
\omega_{2} = 2[(2*0 + 1)(2*0+1)d^{0}_{0,0}*d^{0}_{0,0}*d^{1}_{1,-1}*d^{1}_{1,-1}] \\
 \\ 
A'_{3} = |A_{1}|^2[Re(T^{0}_{1,1,0})Re(T^{0}_{1,1,0}) + Im(T^{0}_{1,1,0})Im(T^{0}_{1,1,0})] \\ 
\omega_{3} = 2[(2*0 + 1)(2*0+1)d^{0}_{0,0}*d^{0}_{0,0}*d^{1}_{1,1}*d^{1}_{1,1}] \\
 \\ 
